src/DY.Lib.ComparseGlue.fst
@@ -1,0 +1,80 @@
+module DY.Lib.ComparseGlue
+
+open Comparse
+open DY.Core.Trace.Type
+open DY.Core.Bytes.Type
+open DY.Core.Bytes
+
+instance bytes_like_bytes: bytes_like bytes = {
+  length = length;
+
+  empty = literal_to_bytes FStar.Seq.empty;
+  empty_length = (fun () -> length_literal_to_bytes FStar.Seq.empty);
+  recognize_empty = (fun b ->
+    match bytes_to_literal b with
+    | None -> false
+    | Some lit ->
+      if Seq.length lit = 0 then (
+        assert(lit `FStar.Seq.eq` FStar.Seq.empty);
+        bytes_to_literal_to_bytes b;
+        true
+      ) else (
+        length_literal_to_bytes FStar.Seq.empty;
+        false
+      )
+  );
+
+  concat = concat;
+  concat_length = (fun b1 b2 -> concat_length b1 b2);
+
+  split = split;
+  split_length = (fun b i -> split_length b i);
+
+  split_concat = (fun b1 b2 -> split_concat b1 b2);
+
+  concat_split = (fun b i -> concat_split b i);
+
+  to_nat = (fun b ->
+    match bytes_to_literal b with
+    | None -> None
+    | Some lit ->  (
+      FStar.Endianness.lemma_be_to_n_is_bounded lit;
+      Some (FStar.Endianness.be_to_n lit)
+    )
+  );
+  from_nat = (fun sz n ->
+    literal_to_bytes (FStar.Endianness.n_to_be sz n)
+  );
+
+  from_to_nat = (fun sz n ->
+    literal_to_bytes_to_literal (FStar.Endianness.n_to_be sz n)
+  );
+
+  to_from_nat = (fun b ->
+    bytes_to_literal_to_bytes b
+  );
+}
+
+val bytes_invariant_is_pre_compatible:
+  pr:protocol_preds -> tr:trace ->
+  Lemma
+  (bytes_pre_is_compatible (bytes_invariant pr tr))
+  [SMTPat (bytes_pre_is_compatible (bytes_invariant pr tr))]
+let bytes_invariant_is_pre_compatible pr tr =
+  bytes_pre_is_compatible_intro #bytes (bytes_invariant pr tr)
+    ()
+    (fun b1 b2 -> ())
+    (fun b i -> ())
+    (fun sz n -> ())
+
+val is_publishable_is_pre_compatible:
+  pr:protocol_preds -> tr:trace ->
+  Lemma
+  (bytes_pre_is_compatible (is_publishable pr tr))
+  [SMTPat (bytes_pre_is_compatible (is_publishable pr tr))]
+let is_publishable_is_pre_compatible pr tr =
+  bytes_pre_is_compatible_intro #bytes (is_publishable pr tr)
+    (literal_to_bytes_is_publishable pr tr FStar.Seq.empty)
+    (fun b1 b2 -> concat_preserves_publishability pr tr b1 b2)
+    (fun b i -> split_preserves_publishability pr tr b i)
+    (fun sz n -> literal_to_bytes_is_publishable pr tr (FStar.Endianness.n_to_be sz n))
